src/Zulib/fstar/Zen.Types.Extracted.fst
@@ -5,12 +5,6 @@ module      V = Zen.Vector
 module     U8 = FStar.UInt8
 module    U32 = FStar.UInt32
 module    U64 = FStar.UInt64
-module Realized = Zen.Types.Realized
-
-type lockCore = Realized.lockCore
-type contract = Realized.contract
-type extendedContract = Realized.extendedContract
-type extraData = Realized.extraData
 
 type byte = U8.byte
 type opcode = U8.t
@@ -19,22 +13,35 @@ type signature = A.t U8.byte 64
 type key       = A.t U8.byte 64
 type asset = hash
 type contractHash = hash
-type spend = {asset: asset; amount: U64.t}
-type outpoint = {txHash: hash; index: U32.t}
 type witness (n:nat) = A.t byte n
-type nonce = A.t byte 64
+type nonce = U64.t * U64.t
+
+type outpoint =
+    { txHash: hash;
+      index: U32.t }
+
+type spend =
+    { asset: asset;
+      amount: U64.t }
+
+type lock =
+    | PKLock of hash
+    | ContractLock of contractHash
+    | DestroyLock
+
+type output =
+    { lock: lock;
+      spend: spend }
+
 
 unopteq type blockHeader = {
     version: U32.t;
     parent: hash;
     blockNumber: U32.t;
-    txMerkleRoot: hash;
-    witnessMerkleRoot: hash;
-    contractMerkleRoot: hash;
-    extraData: extraData;
-    timestamp: FStar.Int64.t;
-    pdiff: U32.t;
-    nonce: nonce
+    commitments: hash;
+    timestamp: U64.t;
+    difficulty: U32.t;
+    nonce: nonce;
     }
 
 noeq type data : nat -> Type =
@@ -45,7 +52,6 @@ noeq type data : nat -> Type =
   | Key: v:key -> data 1
   | Outpoint: v:outpoint -> data 1
   | Output: v:output -> data 1
-  | OutputLock: v:outputLock -> data 1
   | Sig: v:signature -> data 1
   | UInt8 : v:U8.t -> data 1
   | UInt32: v:U32.t -> data 1
@@ -64,8 +70,6 @@ noeq type data : nat -> Type =
   | OutpointArray:  l:nat -> a: A.t outpoint l -> data l
   | OutputVector: l:nat -> v: V.t output l -> data l
   | OutputArray:  l:nat -> a: A.t output l -> data l
-  | OutputLockVector: l:nat -> v: V.t outputLock l -> data l
-  | OutputLockArray:  l:nat -> a: A.t outputLock l -> data l
   | UInt8Vector: l:nat -> v: V.t U8.t l -> data l
   | UInt8Array:  l:nat -> a: A.t U8.t l -> data l
   | UInt32Vector: l:nat -> v: V.t U32.t l -> data l
@@ -77,81 +81,6 @@ noeq type data : nat -> Type =
   | Data3: n1:nat -> n2:nat -> n3:nat -> _1:data n1 -> _2:data n2 -> _3:data n3 -> data (n1+n2+n3)
   | Data4: n1:nat -> n2:nat -> n3:nat -> n4:nat -> _1:data n1 -> _2:data n2 -> _3:data n3 -> _4:data n4 -> data (n1+n2+n3+n4)
 
-(*
-and dataContainer : nat -> Type =
-  | Single: n:nat -> v:data n -> dataContainer n
-  | Data2: n1:nat -> n2:nat -> _1:data n1 -> _2:data n2 -> dataContainer (n1+n2)
-  | Data3: n1:nat -> n2:nat -> n3:nat -> _1:data n1 -> _2:data n2 -> _3:data n3 -> dataContainer (n1+n2+n3)
-  | Data4: n1:nat -> n2:nat -> n3:nat -> n4:nat _1:data n1 -> _2:data n2 -> _3:data n3 -> _4:data n4 -> dataContainer (n1+n2+n3+n4)
-  | Cont2: _1:dataContainer -> _2:dataContainer -> dataContainer
-  | Cont3: _1:dataContainer -> _2:dataContainer -> _3:dataContainer -> dataContainer
-  | Cont4: _1:dataContainer -> _2:dataContainer -> _3:dataContainer -> _4:dataContainer -> dataContainer
-//noeq type lockCore (n:nat) = {version: U32.t; lockData: list (A.t  byte n)}
-*)
-
-and outputLock =
-  | CoinbaseLock of lockCore
-  | FeeLock of lockCore
-  | ContractSacrificeLock of lockCore
-  | PKLock of pkHash: hash
-  | ContractLock: contractHash:hash -> n:nat -> data n -> outputLock
-  | HighVLock: lockcore:lockCore -> typeCode:nat -> outputLock
-and output = {lock: outputLock; spend: spend}
 type inputData (n:nat) = data n
 
-type pointedOutput = outpoint * output
-
-unopteq type transactionSkeleton = | Tx: #l1:nat -> inputs : V.t pointedOutput l1
-                                      -> #l2:nat -> outputs: V.t output l2
-                                      -> option (l3:nat & data l3)
-                                      -> transactionSkeleton
-
 type utxo = outpoint -> option output
-
-unopteq type inputMsg = {
-  cmd: opcode;
-  data: n:nat & inputData n;
-  contractHash: hash;
-  utxo: utxo
-}
-
-
-val maxCost: nat
-let maxCost = 200
-
-noeq type costFunction = | CostFunc: #n:nat{n<=maxCost} -> f:(transactionSkeleton -> Zen.Cost.t nat n) -> costFunction
-
-noeq type mainFunction =
-  | MainFunc: cf:costFunction
-           -> mf: ( inTxSkel:transactionSkeleton
-                    -> Zen.Cost.t (result transactionSkeleton)
-                                  (Zen.Cost.force ((CostFunc?.f cf) inTxSkel))
-                  )
-           -> mainFunction
-
-//val contractVersion : extendedContract -> U32.t
-
-//let contractHashBytes = 32ul
-//let pubKeyHashBytes = 32ul
-//let txHashBytes = 32ul
-
-//type Transaction = {version: uint32; inputs: Outpoint list; witnesses: Witness list; outputs: Output list; contract: Contract option}
-(*
-type transaction = {version: U32.t;
-  inputs: list outpoint;
-  witnesses: list witness;
-  outputs: list output;
-  contract: option extendedContract}
-*)
-
-//type contractContext = {contractId: byte[]; utxo: Map<outpoint, output>; tip: blockHeader; }
-
-//TODO: Review merkleData
-//val merkleData : blockHeader -> list
-
-(*
-type block = {
-    header: blockHeader;
-    transactions: transaction list
-    }
-*)
