src/Zulib/fstar/Zen.Types.Main.fst
@@ -1,0 +1,21 @@
+module Zen.Types.Main
+
+open Zen.Types.TxSkeleton
+open Zen.Types.Extracted
+
+val maxCost: nat
+let maxCost = 200
+
+noeq type costFunction =
+    | CostFunc:
+        #n:nat{n<=maxCost}
+        -> f:(txSkeleton -> Zen.Cost.t nat n)
+        -> costFunction
+
+noeq type mainFunction =
+    | MainFunc:
+        cf:costFunction
+        -> mf:(txSkel:txSkeleton
+                -> Zen.Cost.t (result txSkeleton)
+                              (Zen.Cost.force ((CostFunc?.f cf) txSkel)))
+        -> mainFunction
